modal.v
@@ -1,0 +1,145 @@
+From Coq Require Export Bool.
+From Coq Require Export Relations.
+From Coq Require Export List.
+From Coq Require Export Ensembles.
+From Coq Require Export Relations.
+
+Module Modal.
+
+Definition var := nat.
+
+Inductive Form : Type :=
+  | F_
+  | Var (v : var)
+  | Impl (f1 : Form) (f2 : Form)
+  | Box (f : Form).
+
+Definition Neg (f : Form) := Impl f F_.
+
+Definition Disj (f1 f2 : Form) := Impl (Neg f1) f2.
+
+Definition Conj (f1 f2 : Form) := Neg (Disj (Neg f1) (Neg f2)).
+
+Definition Diamond (f : Form) := Neg (Box (Neg f)).
+
+Search Ensemble.
+
+Section Kripke_Frame.
+
+Variable X : Type.
+
+Structure model := {
+  world : Ensemble X;
+  rel : relation X;
+  val: X -> Ensemble X;
+  eq : equiv X rel
+}.
+
+Record model1 : Type := Model {
+  state :> Type;
+  trans : state -> state -> Prop;
+  label : state -> var -> Prop;
+  eq1 : forall x y z : state, trans x x /\ ((trans x y /\ trans y z) -> trans x z) /\ trans x y -> trans y x;
+  (* dec : forall x : Type, x -> True \/ x -> False *)
+}.
+
+(*  @Verification of Dynamic Bisimulation Theorems in Coq
+    @ Fervari, Trucco, Ziliani
+
+From Mtac2 Require Export Mtac2.
+From Coq.Sets Require Export Constructive_sets.
+From Coq.Relations Require Export Relations.
+From Coq.Logic Require Export Classical.
+From Coq.Lists Require Export List.
+From RCLIC Require Export utilities.
+From mathcomp Require Export ssreflect ssrnat ssrbool eqtype.
+
+Definition valuation (W: Set) : Type := set (prop * W).
+
+Structure model := {
+  m_states :> Set;
+  m_rel : relation m_states;
+  m_val: valuation m_states
+}.
+
+*)
+
+(* @Doczkal & Smolka, 2011 (for K)*)
+Record model2 := Model2 {
+  state2 :> Type;
+  trans2 : state2 -> state2 -> Prop;
+  label2 : var -> (state2 -> Prop);
+  BOX : (state2 -> Prop) -> (state2 -> Prop);
+  boxE : forall p w, BOX p w <-> forall v, trans2 w v -> p v;
+  DIA : (state2 -> Prop) -> (state2 -> Prop);
+  diaE : forall p w, DIA p w <-> exists v, trans2 w v /\ p v;
+}.
+
+
+End Kripke_Frame.
+
+Type world.
+
+(*
+f : X -> bool
+x : X
+g y = if x = y then true else f y
+*)
+
+
+Definition implies (b1:bool) (b2:bool) : bool :=
+  match b1 with
+  | true => b2
+  | false => true
+  end.
+
+Definition neg (b:bool) : bool := implies b false.
+
+Definition and (b1:bool) (b2:bool) : bool := neg (implies b1 (neg b2)).
+
+Definition or (b1:bool) (b2:bool) : bool := implies (neg b1) b2.
+
+Definition ifonlyif (b1:bool) (b2:bool) : bool :=
+  and (implies b1 b2) (implies b2 b1).
+
+Search relation.
+
+Fixpoint interpret (f : Form) (m : model1) (w : state m) (i : model1 -> state m -> var -> bool) : bool :=
+  match f with
+  | F_ => false
+  | Var x => i m w x
+  | Impl f1 f2 => implies (interpret f1 m w i) (interpret f2 m w i)
+  | Box f => true
+(*  | Box f => forall x y : state m, trans m x y -> interpretP f m w i *)
+  end.
+
+Fixpoint interpretP (f : Form) (m : model1) (w : state m) (i : model1 -> state m -> var -> bool) : Prop :=
+  match f with
+  | F_ => Is_true (interpret f m w i)
+  | Var x => Is_true (interpret f m w i)
+  | Impl f1 f2 => Is_true (interpret f m w i)
+  | Box f => forall x y : state m, trans m x y -> interpretP f m w i 
+  end.
+
+Inductive ax_s5 : Form -> Prop :=
+  | a_1 (x y : Form) : ax_s5 (Impl x (Impl y x))
+  | a_2 (x y z : Form) : ax_s5 (Impl (Impl x (Impl y z)) (Impl (Impl x y) (Impl x z)))
+  | a_3 (x y : Form) : ax_s5 (Impl (Impl (Neg x) (Neg y)) (Impl y x))
+  | a_k (x y : Form) : ax_s5 (Impl (Box (Impl x y)) (Impl (Box x) (Box y)))
+  | a_t (x : Form) : ax_s5 (Impl (Box x) x)
+  | a_4 (x : Form) : ax_s5 (Impl (Box x) (Box (Box x)))
+  | a_b (x : Form) : ax_s5 (Impl x (Box (Diamond x)))
+  | mp (x y z : Form) : ax_s5 (Impl x y) -> ax_s5 x -> ax_s5 y
+  | nec (x : Form) : ax_s5 x -> ax_s5 (Box x).
+
+Lemma ax_s5_sound (x : Form) :
+  ax_s5 x -> forall m w i, interpretP x m w i.
+Proof.
+  intros H. induction H.
+Admitted.
+(* Qed. *)
+
+End Modal.
+
+
+
